LiveVerif/src/LiveVerif/LiveProgramLogic.v
@@ -794,7 +794,7 @@ Ltac with_ident_as_string_no_beta f :=
 Declare Custom Entry funspec.
 
 (* One return value: *)
-Notation "'uintptr_t' fname ( 'uintptr_t' a1 , 'uintptr_t' .. , 'uintptr_t' an ) /**# 'ghost_args' := g1 .. gn ; 'requires' t1 m1 := pre ; 'ensures' t2 m2 r := post #* */ /* *" :=
+Notation "'uintptr_t' fname ( 'uintptr_t' a1 , 'uintptr_t' .. , 'uintptr_t' an ) /* *# 'ghost_args' := g1 .. gn ; 'requires' t1 m1 := pre ; 'ensures' t2 m2 r := post #* */ /* *" :=
   (fun fname: String.string =>
      (fun fs =>
         (forall a1, .. (forall an, (forall g1, .. (forall gn,
@@ -813,7 +813,7 @@ Notation "'uintptr_t' fname ( 'uintptr_t' a1 , 'uintptr_t' .. , 'uintptr_t' an )
  only parsing).
 
 (* No return value: *)
-Notation "'void' fname ( 'uintptr_t' a1 , 'uintptr_t' .. , 'uintptr_t' an ) /**# 'ghost_args' := g1 .. gn ; 'requires' t1 m1 := pre ; 'ensures' t2 m2 := post #* */ /* *" :=
+Notation "'void' fname ( 'uintptr_t' a1 , 'uintptr_t' .. , 'uintptr_t' an ) /* *# 'ghost_args' := g1 .. gn ; 'requires' t1 m1 := pre ; 'ensures' t2 m2 := post #* */ /* *" :=
   (fun fname: String.string =>
      (fun fs =>
         (forall a1, .. (forall an, (forall g1, .. (forall gn,
